src/Init/Data/Range/Polymorphic/Lemmas.lean
@@ -90,6 +90,13 @@ theorem PRange.UpwardEnumerable.exists_of_succ_le [UpwardEnumerable α] [LawfulU
   rw [succMany?_eq_some_iff_succMany, succMany_succ_eq_succ_succMany] at hn
   exact ⟨succMany n a, hn.symm, ⟨n, succMany?_eq_some⟩⟩
 
+theorem PRange.UpwardEnumerable.exists_of_succ_lt [UpwardEnumerable α] [LawfulUpwardEnumerable α]
+    [InfinitelyUpwardEnumerable α] {a b : α} (h : UpwardEnumerable.LT (succ a) b) :
+    ∃ b', b = succ b' ∧ UpwardEnumerable.LT a b' := by
+  obtain ⟨n, hn⟩ := h
+  rw [succMany?_eq_some_iff_succMany, succMany_succ_eq_succ_succMany] at hn
+  exact ⟨succMany (n + 1) a, hn.symm, ⟨n, succMany?_eq_some⟩⟩
+
 private theorem Rcc.Internal.forIn'_eq_forIn'_iter [LE α] [DecidableLE α] [UpwardEnumerable α]
     [LawfulUpwardEnumerableLE α] [Rxc.IsAlwaysFinite α] [LawfulUpwardEnumerable α]
     {γ : Type u} {init : γ} {m : Type u → Type w} [Monad m] {r : Rcc α}
@@ -162,9 +169,8 @@ private theorem Roo.Internal.forIn'_eq_forIn'_iter [LT α] [DecidableLT α]
       ForIn'.forIn' (Internal.iter r) init (fun a ha acc => f a (Internal.isPlausibleIndirectOutput_iter_iff.mp ha) acc) := by
   rfl
 
-private theorem Roo.Internal.toList_eq_toList_iter [LE α] [LT α] [DecidableLT α]
-    [UpwardEnumerable α] [Rxo.IsAlwaysFinite α] [LawfulUpwardEnumerable α]
-    [LawfulUpwardEnumerableLE α] {r : Roo α} :
+private theorem Roo.Internal.toList_eq_toList_iter [LT α] [DecidableLT α]
+    [UpwardEnumerable α] [Rxo.IsAlwaysFinite α] [LawfulUpwardEnumerable α] {r : Roo α} :
     r.toList = (Internal.iter r).toList := by
   rfl
 
@@ -178,7 +184,7 @@ private theorem Roi.Internal.forIn'_eq_forIn'_iter [LT α] [DecidableLT α]
       ForIn'.forIn' (Internal.iter r) init (fun a ha acc => f a (Internal.isPlausibleIndirectOutput_iter_iff.mp ha) acc) := by
   rfl
 
-private theorem Roi.Internal.toList_eq_toList_iter [LE α]
+private theorem Roi.Internal.toList_eq_toList_iter
     [UpwardEnumerable α] [Rxi.IsAlwaysFinite α] [LawfulUpwardEnumerable α] {r : Roi α} :
     r.toList = (Internal.iter r).toList := by
   rfl
@@ -1015,6 +1021,635 @@ public theorem isEmpty_iff_forall_not_mem [LE α] [UpwardEnumerable α]
   exact ⟨r.lower, by simpa [← UpwardEnumerable.le_iff] using UpwardEnumerable.le_refl (α := α) _⟩
 
 end Rci
+
+namespace Roc
+
+variable {r : Roc α}
+
+public theorem toList_eq_match [LE α] [DecidableLE α] [UpwardEnumerable α]
+    [LawfulUpwardEnumerable α] [LawfulUpwardEnumerableLE α] [Rxc.IsAlwaysFinite α]
+    [LawfulUpwardEnumerable α] :
+    r.toList = match UpwardEnumerable.succ? r.lower with
+      | none => []
+      | some next =>
+        if next ≤ r.upper then
+          next :: (next<...=r.upper).toList
+        else
+          [] := by
+  rw [Internal.toList_eq_toList_iter, Rxc.Iterator.toList_eq_match (it := Internal.iter r)]
+  simp [Internal.iter, Internal.toList_eq_toList_iter]
+
+public theorem toList_eq_nil_iff [LE α] [DecidableLE α] [LT α] [UpwardEnumerable α]
+    [LawfulUpwardEnumerable α] [LawfulUpwardEnumerableLE α] [LawfulUpwardEnumerableLT α]
+    [Rxc.IsAlwaysFinite α] [LawfulUpwardEnumerable α] :
+    r.toList = [] ↔ ¬ (r.lower < r.upper) := by
+  rw [Internal.toList_eq_toList_iter, Rxc.Iterator.toList_eq_match, Internal.iter]
+  simp only
+  split <;> rename_i heq <;>
+    simp [UpwardEnumerable.lt_iff, UpwardEnumerable.lt_iff_exists,
+      UpwardEnumerable.le_iff, UpwardEnumerable.le_iff_exists,
+      UpwardEnumerable.succMany?_succ?_eq_succ?_bind_succMany?, heq]
+
+public theorem mem_toList_iff_mem [LE α] [DecidableLE α] [LT α] [DecidableLT α] [UpwardEnumerable α]
+    [LawfulUpwardEnumerable α] [LawfulUpwardEnumerableLE α] [LawfulUpwardEnumerableLT α]
+    [Rxc.IsAlwaysFinite α] [LawfulUpwardEnumerable α] {a : α} : a ∈ r.toList ↔ a ∈ r := by
+  rw [Internal.toList_eq_toList_iter, Iter.mem_toList_iff_isPlausibleIndirectOutput,
+    Internal.isPlausibleIndirectOutput_iter_iff]
+
+public theorem pairwise_toList_upwardEnumerableLt [LE α] [DecidableLE α]
+    [UpwardEnumerable α] [LawfulUpwardEnumerable α] [LawfulUpwardEnumerableLE α]
+    [Rxc.IsAlwaysFinite α] [LawfulUpwardEnumerable α] :
+    r.toList.Pairwise (fun a b => UpwardEnumerable.LT a b) := by
+  rw [Internal.toList_eq_toList_iter]
+  apply Rxc.Iterator.pairwise_toList_upwardEnumerableLt
+
+public theorem pairwise_toList_ne [LE α] [DecidableLE α]
+    [UpwardEnumerable α] [LawfulUpwardEnumerable α] [LawfulUpwardEnumerableLE α]
+    [Rxc.IsAlwaysFinite α] [LawfulUpwardEnumerable α] :
+    r.toList.Pairwise (fun a b => a ≠ b) :=
+  List.Pairwise.imp (fun hlt => UpwardEnumerable.ne_of_lt hlt) pairwise_toList_upwardEnumerableLt
+
+public theorem pairwise_toList_lt [LE α] [DecidableLE α] [LT α]
+    [UpwardEnumerable α] [LawfulUpwardEnumerable α] [LawfulUpwardEnumerableLE α]
+    [LawfulUpwardEnumerableLT α] [Rxc.IsAlwaysFinite α] [LawfulUpwardEnumerable α] :
+    r.toList.Pairwise (fun a b => a < b) :=
+  List.Pairwise.imp
+    (fun hlt => (LawfulUpwardEnumerableLT.lt_iff ..).mpr hlt) pairwise_toList_upwardEnumerableLt
+
+public theorem pairwise_toList_le [LE α] [DecidableLE α] [LT α]
+    [UpwardEnumerable α] [LawfulUpwardEnumerable α] [LawfulUpwardEnumerableLE α]
+    [Rxc.IsAlwaysFinite α] [LawfulUpwardEnumerable α] :
+    r.toList.Pairwise (fun a b => a ≤ b) :=
+  pairwise_toList_upwardEnumerableLt
+    |> List.Pairwise.imp UpwardEnumerable.le_of_lt
+    |> List.Pairwise.imp (fun hle => (UpwardEnumerable.le_iff ..).mpr hle)
+
+public theorem mem_succ_succ_iff [LE α] [DecidableLE α] [LT α] [UpwardEnumerable α]
+    [LinearlyUpwardEnumerable α] [LawfulUpwardEnumerableLE α] [LawfulUpwardEnumerableLT α]
+    [InfinitelyUpwardEnumerable α] [Rxc.IsAlwaysFinite α] [LawfulUpwardEnumerable α] {lo hi a : α} :
+    (a ∈ (succ lo)<...=(succ hi)) ↔ ∃ a', a = succ a' ∧ a' ∈ lo<...=hi := by
+  simp [Membership.mem, UpwardEnumerable.le_iff, UpwardEnumerable.lt_iff]
+  constructor
+  · intro h
+    obtain ⟨a', rfl, ha'⟩ := UpwardEnumerable.exists_of_succ_lt h.1
+    exact ⟨a', rfl, ha', UpwardEnumerable.succ_le_succ_iff.mp h.2⟩
+  · rintro ⟨a', rfl, hl, hu⟩
+    exact ⟨UpwardEnumerable.succ_lt_succ_iff.mpr hl, UpwardEnumerable.succ_le_succ_iff.mpr hu⟩
+
+public theorem succ_mem_succ_succ_iff [LE α] [DecidableLE α] [LT α] [UpwardEnumerable α]
+    [LinearlyUpwardEnumerable α] [LawfulUpwardEnumerableLE α] [LawfulUpwardEnumerableLT α]
+    [InfinitelyUpwardEnumerable α]
+    [Rxc.IsAlwaysFinite α] [LawfulUpwardEnumerable α] {lo hi a : α} :
+    (succ a ∈ (succ lo)<...=(succ hi)) ↔ a ∈ lo<...=hi := by
+  simp [mem_succ_succ_iff, UpwardEnumerable.succ_inj]
+
+public theorem toList_succ_succ_eq_map [LE α] [DecidableLE α] [LT α] [DecidableLT α]
+    [UpwardEnumerable α] [LinearlyUpwardEnumerable α] [LawfulUpwardEnumerableLE α]
+    [LawfulUpwardEnumerableLT α] [InfinitelyUpwardEnumerable α] [Rxc.IsAlwaysFinite α]
+    [LawfulUpwardEnumerable α] {lo hi : α} :
+    ((succ lo)<...=(succ hi)).toList =
+      (lo<...=hi).toList.map succ := by
+  apply eq_of_pairwise_lt_of_mem_iff_mem (lt := UpwardEnumerable.LT)
+  · exact pairwise_toList_upwardEnumerableLt
+  · apply List.Pairwise.map (R := UpwardEnumerable.LT) (S := UpwardEnumerable.LT)
+    · exact fun _ _ => UpwardEnumerable.succ_lt_succ_iff.mpr
+    · exact pairwise_toList_upwardEnumerableLt
+  · simp [List.mem_map, mem_toList_iff_mem, mem_succ_succ_iff, eq_comm, and_comm]
+
+public theorem forIn'_eq_forIn'_toList [LE α] [DecidableLE α] [LT α] [DecidableLT α]
+    [UpwardEnumerable α] [LawfulUpwardEnumerableLE α] [LawfulUpwardEnumerableLT α]
+    [Rxc.IsAlwaysFinite α] [LawfulUpwardEnumerable α] {γ : Type u} {init : γ} {m : Type u → Type w}
+    [Monad m] [LawfulMonad m] {f : (a : α) → a ∈ r → γ → m (ForInStep γ)} :
+    ForIn'.forIn' r init f =
+      ForIn'.forIn' r.toList init (fun a ha acc => f a (mem_toList_iff_mem.mp ha) acc) := by
+  simp [Internal.forIn'_eq_forIn'_iter, Internal.toList_eq_toList_iter,
+    Iter.forIn'_eq_forIn'_toList]
+
+public theorem forIn'_toList_eq_forIn' [LE α] [DecidableLE α] [LT α] [DecidableLT α] [UpwardEnumerable α]
+    [LawfulUpwardEnumerableLE α] [LawfulUpwardEnumerableLT α] [Rxc.IsAlwaysFinite α]
+    [LawfulUpwardEnumerable α] {γ : Type u} {init : γ} {m : Type u → Type w} [Monad m]
+    [LawfulMonad m] {f : (a : α) → _ → γ → m (ForInStep γ)} :
+    ForIn'.forIn' r.toList init f =
+      ForIn'.forIn' r init (fun a ha acc => f a (mem_toList_iff_mem.mpr ha) acc) := by
+  simp [forIn'_eq_forIn'_toList]
+
+public theorem mem_of_mem_of_le [LE α] [LT α] [UpwardEnumerable α] [LawfulUpwardEnumerable α]
+    [LawfulUpwardEnumerableLE α] [LawfulUpwardEnumerableLT α] {lo lo' hi a : α}
+    (h : lo ≤ lo') (hmem : a ∈ lo'<...=hi) :
+    a ∈ lo<...=hi := by
+  simp only [Membership.mem, UpwardEnumerable.le_iff, UpwardEnumerable.lt_iff] at h hmem ⊢
+  exact ⟨UpwardEnumerable.lt_of_le_of_lt h hmem.1, hmem.2⟩
+
+-- public theorem SupportsLowerBound.isSatisfied_init? {sl} [UpwardEnumerable α]
+--     [SupportsLowerBound sl α] [BoundedUpwardEnumerable sl α] [LawfulUpwardEnumerable α]
+--     [LawfulUpwardEnumerableLowerBound sl α]
+--     {bound : Bound sl α} {a : α} (h : init? bound = some a) :
+--     SupportsLowerBound.IsSatisfied bound a := by
+--   simp only [LawfulUpwardEnumerableLowerBound.isSatisfied_iff]
+--   exact ⟨a, h, UpwardEnumerable.le_refl _⟩
+
+public theorem forIn'_eq_match_Roc [LE α] [DecidableLE α] [LT α] [DecidableLT α]
+    [UpwardEnumerable α] [LawfulUpwardEnumerableLT α] [LawfulUpwardEnumerableLE α]
+    [Rxc.IsAlwaysFinite α] [LawfulUpwardEnumerable α]
+    {m : Type u → Type w} [Monad m] [LawfulMonad m]
+    {γ : Type u} {init : γ} {f : (a : α) → _ → γ → m (ForInStep γ)} :
+    ForIn'.forIn' r init f = match hs : UpwardEnumerable.succ? r.lower with
+      | none => return init
+      | some next =>
+        if hu : next ≤ r.upper then do
+          have hlt : r.lower < next :=
+            UpwardEnumerable.lt_iff.mpr ⟨0, by simpa [UpwardEnumerable.succMany?_one] using hs⟩
+          match ← f next ⟨hlt, hu⟩ init with
+          | .yield c =>
+            haveI := UpwardEnumerable.instLawfulOrderLTOfLawfulUpwardEnumerableLT (α := α)
+            ForIn'.forIn' (α := α) (β := γ) (next<...=r.upper) c
+              (fun a ha acc => f a (mem_of_mem_of_le (le_of_lt hlt) ha) acc)
+          | .done c => return c
+      else
+        return init := by
+  apply Eq.symm
+  rw [Internal.forIn'_eq_forIn'_iter, Iter.forIn'_eq_match_step]
+  simp only [Rxc.Iterator.step_eq_step, Rxc.Iterator.step, Internal.iter]
+  split <;> rename_i heq
+  · simp [heq]
+  · split <;> rename_i heq'
+    · simp only [Internal.forIn'_eq_forIn'_iter, Internal.iter, ↓reduceIte, heq', heq]
+      apply bind_congr; intro step
+      split <;> simp
+    · simp [heq, heq']
+
+public theorem isEmpty_iff_forall_not_mem [LE α] [LT α] [DecidableLT α] [UpwardEnumerable α]
+    [Rxc.HasSize α] [Rxc.LawfulHasSize α] [LawfulUpwardEnumerableLE α]
+    [LawfulUpwardEnumerableLT α] [Rxc.IsAlwaysFinite α]
+    [LawfulUpwardEnumerable α] :
+    r.isEmpty ↔ ∀ a, ¬ a ∈ r := by
+  simp only [isEmpty, decide_eq_true_eq]
+  constructor
+  · rintro h a ⟨hl, hu⟩
+    simp only [UpwardEnumerable.le_iff, UpwardEnumerable.lt_iff] at h hl hu
+    exact h.elim (UpwardEnumerable.lt_of_lt_of_le hl hu)
+  · intro h hi
+    refine h r.upper ⟨hi, ?_⟩
+    simpa [UpwardEnumerable.le_iff] using UpwardEnumerable.le_refl _
+
+end Roc
+
+namespace Roo
+
+variable {r : Roo α}
+
+public theorem toList_eq_match [LE α] [LT α] [DecidableLT α] [UpwardEnumerable α]
+    [LawfulUpwardEnumerable α] [LawfulUpwardEnumerableLT α] [Rxo.IsAlwaysFinite α]
+    [LawfulUpwardEnumerable α] :
+    r.toList = match UpwardEnumerable.succ? r.lower with
+      | none => []
+      | some next =>
+        if next < r.upper then
+          next :: (next<...<r.upper).toList
+        else
+          [] := by
+  rw [Internal.toList_eq_toList_iter, Rxo.Iterator.toList_eq_match]; rfl
+
+public theorem toList_eq_nil_iff [LE α] [LT α] [DecidableLT α] [UpwardEnumerable α]
+    [LawfulUpwardEnumerable α] [LawfulUpwardEnumerableLT α] [Rxo.IsAlwaysFinite α]
+    [LawfulUpwardEnumerable α] :
+    r.toList = [] ↔ ∀ a, UpwardEnumerable.succ? r.lower = some a → ¬ (a < r.upper) := by
+  rw [Internal.toList_eq_toList_iter, Rxo.Iterator.toList_eq_match, Internal.iter]
+  simp only
+  split <;> rename_i heq <;> simp [heq]
+
+public theorem mem_toList_iff_mem [LT α] [DecidableLT α] [UpwardEnumerable α]
+    [LawfulUpwardEnumerable α] [LawfulUpwardEnumerableLT α]
+    [Rxo.IsAlwaysFinite α] [LawfulUpwardEnumerable α] {a : α} : a ∈ r.toList ↔ a ∈ r := by
+  rw [Internal.toList_eq_toList_iter, Iter.mem_toList_iff_isPlausibleIndirectOutput,
+    Internal.isPlausibleIndirectOutput_iter_iff]
+
+-- public theorem BoundedUpwardEnumerable.init?_succ?_closed [UpwardEnumerable α]
+--     [LawfulUpwardEnumerable α] {lower lower' : Bound .closed α}
+--     (h : UpwardEnumerable.succ? lower = some lower') :
+--     init? lower' = (init? lower).bind UpwardEnumerable.succ? := by
+--   cases h : init? lower <;> rename_i ilower <;> cases h' : init? lower' <;> rename_i ilower'
+--   · simp
+--   · simp [init?] at h
+--   · simp [init?] at h'
+--   · simp_all [init?]
+
+-- @[deprecated BoundedUpwardEnumerable.init?_succ?_closed (since := "2025-08-22")]
+-- public theorem BoundedUpwardEnumerable.Closed.init?_succ [UpwardEnumerable α]
+--     [LawfulUpwardEnumerable α] {lower lower' : Bound .closed α}
+--     (h : UpwardEnumerable.succ? lower = some lower') :
+--     init? lower' = (init? lower).bind UpwardEnumerable.succ? :=
+--   init?_succ?_closed h
+
+public theorem pairwise_toList_upwardEnumerableLt [LT α] [DecidableLT α]
+    [UpwardEnumerable α] [LawfulUpwardEnumerable α] [LawfulUpwardEnumerableLT α]
+    [Rxo.IsAlwaysFinite α] [LawfulUpwardEnumerable α] :
+    r.toList.Pairwise (fun a b => UpwardEnumerable.LT a b) := by
+  rw [Internal.toList_eq_toList_iter]
+  apply Rxo.Iterator.pairwise_toList_upwardEnumerableLt
+
+public theorem pairwise_toList_ne [LT α] [DecidableLT α]
+    [UpwardEnumerable α] [LawfulUpwardEnumerable α] [LawfulUpwardEnumerableLT α]
+    [Rxo.IsAlwaysFinite α] [LawfulUpwardEnumerable α] :
+    r.toList.Pairwise (fun a b => a ≠ b) :=
+  List.Pairwise.imp (fun hlt => UpwardEnumerable.ne_of_lt hlt) pairwise_toList_upwardEnumerableLt
+
+public theorem pairwise_toList_lt [LT α] [DecidableLT α]
+    [UpwardEnumerable α] [LawfulUpwardEnumerable α] [LawfulUpwardEnumerableLT α]
+    [Rxo.IsAlwaysFinite α] [LawfulUpwardEnumerable α] :
+    r.toList.Pairwise (fun a b => a < b) :=
+  List.Pairwise.imp
+    (fun hlt => (LawfulUpwardEnumerableLT.lt_iff ..).mpr hlt) pairwise_toList_upwardEnumerableLt
+
+public theorem pairwise_toList_le [LE α] [LT α] [DecidableLT α]
+    [UpwardEnumerable α] [LawfulUpwardEnumerable α] [LawfulUpwardEnumerableLT α]
+    [LawfulUpwardEnumerableLE α] [Rxo.IsAlwaysFinite α] [LawfulUpwardEnumerable α] :
+    r.toList.Pairwise (fun a b => a ≤ b) :=
+  pairwise_toList_upwardEnumerableLt
+    |> List.Pairwise.imp UpwardEnumerable.le_of_lt
+    |> List.Pairwise.imp (fun hle => (UpwardEnumerable.le_iff ..).mpr hle)
+
+-- public theorem mem_Roo_succ_succ_iff [LE α] [DecidableLE α] [UpwardEnumerable α]
+--     [LinearlyUpwardEnumerable α] [LawfulUpwardEnumerableLE α] [InfinitelyUpwardEnumerable α]
+--     [HasFiniteRanges .open α] [LawfulUpwardEnumerable α] [LawfulOpenUpperBound α]
+--     {lower : Bound .closed α} {upper : Bound .open α} {a : α} :
+--     (a ∈ (succ lower)...(succ upper)) ↔ ∃ a', a = succ a' ∧ a' ∈ lower...upper := by
+--   simp [Membership.mem, LawfulUpwardEnumerableLowerBound.isSatisfied_iff,
+--     init?, LawfulOpenUpperBound.isSatisfied_iff_le]
+--   rw [← Option.some_get (InfinitelyUpwardEnumerable.isSome_succ? _)]
+--   simp only [Option.some.injEq, ← UpwardEnumerable.succ.eq_def]
+--   simp
+--   constructor
+--   · rintro ⟨⟨n, hn⟩, h⟩
+--     rw [succMany?_eq_some_iff_succMany, ← succMany_one, ← succMany_add, Nat.add_comm, succMany_add,
+--       succMany_one] at hn
+--     rw [← hn]
+--     refine ⟨succMany n lower, rfl, ?_, ?_⟩
+--     · exact ⟨n, by simp [succMany_eq_get]⟩
+--     · obtain ⟨m, hm⟩ := h
+--       refine ⟨m, ?_⟩
+--       rw [succMany?_eq_some_iff_succMany] at hm ⊢
+--       rwa [← hn, ← succMany_one, ← succMany_add, Nat.add_comm, succMany_add, succMany_one,
+--         succ_eq_succ_iff] at hm
+--   · rintro ⟨a', rfl, hl, hu⟩
+--     simp [UpwardEnumerable.succ_le_succ_iff, UpwardEnumerable.succ_lt_succ_iff]
+--     exact ⟨hl, hu⟩
+
+public theorem mem_succ_succ_iff [LT α] [DecidableLT α] [UpwardEnumerable α]
+    [LinearlyUpwardEnumerable α] [LawfulUpwardEnumerableLT α]
+    [InfinitelyUpwardEnumerable α] [Rxo.IsAlwaysFinite α] [LawfulUpwardEnumerable α] {lo hi a : α} :
+    (a ∈ (succ lo)<...(succ hi)) ↔ ∃ a', a = succ a' ∧ a' ∈ lo<...hi := by
+  simp [Membership.mem, UpwardEnumerable.lt_iff]
+  constructor
+  · intro h
+    obtain ⟨a', rfl, ha'⟩ := UpwardEnumerable.exists_of_succ_lt h.1
+    exact ⟨a', rfl, ha', UpwardEnumerable.succ_lt_succ_iff.mp h.2⟩
+  · rintro ⟨a', rfl, hl, hu⟩
+    simp only [UpwardEnumerable.succ_lt_succ_iff]
+    exact ⟨hl, hu⟩
+
+public theorem succ_mem_succ_succ_iff [LT α] [DecidableLT α] [UpwardEnumerable α]
+    [LinearlyUpwardEnumerable α] [LawfulUpwardEnumerableLT α]
+    [InfinitelyUpwardEnumerable α] [Rxo.IsAlwaysFinite α] [LawfulUpwardEnumerable α] {lo hi a : α} :
+    (succ a ∈ (succ lo)<...(succ hi)) ↔ a ∈ lo<...hi := by
+  simp [mem_succ_succ_iff, UpwardEnumerable.succ_inj]
+
+-- public theorem toList_Roo_succ_succ_eq_map [UpwardEnumerable α] [SupportsLowerBound .closed α]
+--     [LinearlyUpwardEnumerable α] [InfinitelyUpwardEnumerable α] [SupportsUpperBound .open α]
+--     [HasFiniteRanges .open α] [LawfulUpwardEnumerable α] [LawfulOpenUpperBound α]
+--     [LawfulUpwardEnumerableLowerBound .closed α] [LawfulUpwardEnumerableUpperBound .open α]
+--     {lower : Bound .closed α} {upper : Bound .open α} :
+--     ((succ lower)...(succ upper)).toList =
+--       (lower...upper).toList.map succ := by
+--   apply eq_of_pairwise_lt_of_mem_iff_mem (lt := UpwardEnumerable.LT) (asymm := ?_)
+--   · apply pairwise_toList_upwardEnumerableLt
+--   · apply List.Pairwise.map (R := UpwardEnumerable.LT) (S := UpwardEnumerable.LT)
+--     · intro a b
+--       exact UpwardEnumerable.succ_lt_succ_iff.mpr
+--     · apply pairwise_toList_upwardEnumerableLt
+--   · simp only [List.mem_map, mem_toList_iff_mem]
+--     intro a
+--     rw [mem_Roo_succ_succ_iff]
+--     constructor
+--     · rintro ⟨a, rfl, h⟩
+--       exact ⟨a, h, rfl⟩
+--     · rintro ⟨a, h, h'⟩
+--       exact ⟨_, h'.symm, h⟩
+--   · exact ⟨fun _ _ => UpwardEnumerable.not_gt_of_lt⟩
+
+public theorem toList_succ_succ_eq_map [LT α] [DecidableLT α]
+    [UpwardEnumerable α] [LinearlyUpwardEnumerable α]
+    [LawfulUpwardEnumerableLT α] [InfinitelyUpwardEnumerable α] [Rxo.IsAlwaysFinite α]
+    [LawfulUpwardEnumerable α] {lo hi : α} :
+    ((succ lo)<...(succ hi)).toList =
+      (lo<...hi).toList.map succ := by
+  apply eq_of_pairwise_lt_of_mem_iff_mem (lt := UpwardEnumerable.LT)
+  · exact pairwise_toList_upwardEnumerableLt
+  · apply List.Pairwise.map (R := UpwardEnumerable.LT) (S := UpwardEnumerable.LT)
+    · exact fun _ _ => UpwardEnumerable.succ_lt_succ_iff.mpr
+    · exact pairwise_toList_upwardEnumerableLt
+  · simp [List.mem_map, mem_toList_iff_mem, mem_succ_succ_iff, eq_comm, and_comm]
+
+public theorem forIn'_eq_forIn'_toList [LT α] [DecidableLT α]
+    [UpwardEnumerable α] [LawfulUpwardEnumerableLT α]
+    [Rxo.IsAlwaysFinite α] [LawfulUpwardEnumerable α]
+    {γ : Type u} {init : γ} {m : Type u → Type w} [Monad m] [LawfulMonad m]
+    {f : (a : α) → a ∈ r → γ → m (ForInStep γ)} :
+    ForIn'.forIn' r init f =
+      ForIn'.forIn' r.toList init (fun a ha acc => f a (mem_toList_iff_mem.mp ha) acc) := by
+  simp [Internal.forIn'_eq_forIn'_iter, Internal.toList_eq_toList_iter,
+    Iter.forIn'_eq_forIn'_toList]
+
+public theorem forIn'_toList_eq_forIn' [LT α] [DecidableLT α]
+    [UpwardEnumerable α] [LawfulUpwardEnumerableLT α]
+    [Rxo.IsAlwaysFinite α] [LawfulUpwardEnumerable α]
+    {γ : Type u} {init : γ} {m : Type u → Type w} [Monad m] [LawfulMonad m]
+    {f : (a : α) → _ → γ → m (ForInStep γ)} :
+    ForIn'.forIn' r.toList init f =
+      ForIn'.forIn' r init (fun a ha acc => f a (mem_toList_iff_mem.mpr ha) acc) := by
+  simp [forIn'_eq_forIn'_toList]
+
+public theorem mem_of_mem_of_le [LT α] [UpwardEnumerable α]
+    [LawfulUpwardEnumerableLT α] [Rxo.IsAlwaysFinite α]
+    [LawfulUpwardEnumerable α] {a b : α} (hrb : UpwardEnumerable.LE r.lower b)
+    (hmem : a ∈ b<...r.upper) : a ∈ r := by
+  refine ⟨UpwardEnumerable.lt_iff.mpr (UpwardEnumerable.lt_of_le_of_lt hrb ?_), hmem.2⟩
+  exact UpwardEnumerable.lt_iff.mp hmem.1
+
+-- public theorem SupportsLowerBound.isSatisfied_init? {sl} [UpwardEnumerable α]
+--     [SupportsLowerBound sl α] [BoundedUpwardEnumerable sl α] [LawfulUpwardEnumerable α]
+--     [LawfulUpwardEnumerableLowerBound sl α]
+--     {bound : Bound sl α} {a : α} (h : init? bound = some a) :
+--     SupportsLowerBound.IsSatisfied bound a := by
+--   simp only [LawfulUpwardEnumerableLowerBound.isSatisfied_iff]
+--   exact ⟨a, h, UpwardEnumerable.le_refl _⟩
+
+public theorem forIn'_eq_match_Roo [LT α] [DecidableLT α]
+    [UpwardEnumerable α] [LawfulUpwardEnumerableLT α]
+    [Rxo.IsAlwaysFinite α] [LawfulUpwardEnumerable α]
+    {m : Type u → Type w} [Monad m] [LawfulMonad m]
+    {γ : Type u} {init : γ} {f : (a : α) → _ → γ → m (ForInStep γ)} :
+    ForIn'.forIn' r init f = match hs : UpwardEnumerable.succ? r.lower with
+      | none => return init
+      | some next =>
+        if hu : next < r.upper then do
+          have hlt : r.lower < next :=
+            UpwardEnumerable.lt_iff.mpr ⟨0, by simpa [UpwardEnumerable.succMany?_one] using hs⟩
+          have hle : UpwardEnumerable.LE r.lower next :=
+            ⟨1, by simpa [UpwardEnumerable.succMany?_one] using hs⟩
+          match ← f next ⟨hlt, hu⟩ init with
+          | .yield c =>
+            ForIn'.forIn' (α := α) (β := γ) (next<...r.upper) c
+              (fun a ha acc => f a (mem_of_mem_of_le hle ha) acc)
+          | .done c => return c
+      else
+        return init := by
+  apply Eq.symm
+  rw [Internal.forIn'_eq_forIn'_iter, Iter.forIn'_eq_match_step]
+  simp only [Rxo.Iterator.step_eq_step, Rxo.Iterator.step, Internal.iter]
+  split <;> rename_i heq
+  · simp [heq]
+  · split <;> rename_i heq'
+    · simp only [Internal.forIn'_eq_forIn'_iter, Internal.iter, ↓reduceIte, heq', heq]
+      apply bind_congr; intro step
+      split <;> rfl
+    · simp [heq, heq']
+
+public theorem isEmpty_iff_forall_not_mem [LT α] [DecidableLT α] [UpwardEnumerable α]
+    [Rxo.HasSize α] [Rxo.LawfulHasSize α]
+    [LawfulUpwardEnumerableLT α] [Rxo.IsAlwaysFinite α]
+    [LawfulUpwardEnumerable α] :
+    r.isEmpty ↔ ∀ a, ¬ a ∈ r := by
+  simp only [isEmpty, decide_eq_true_eq]
+  constructor
+  · rintro h a ⟨hl, hu⟩
+    simp only [UpwardEnumerable.lt_iff, UpwardEnumerable.lt_iff] at h hl hu
+    obtain ⟨n, hn⟩ := hl
+    simp only [succMany?_succ?_eq_succ?_bind_succMany?, Option.bind_eq_some_iff] at hn
+    obtain ⟨a', ha', hn⟩ := hn
+    exact h a' ha' (UpwardEnumerable.lt_of_le_of_lt ⟨n, hn⟩ hu)
+  · intro h a ha
+    exact (h a).imp fun hu =>
+      ⟨UpwardEnumerable.lt_iff.mpr ⟨0, by simpa [UpwardEnumerable.succMany?_one]⟩, hu⟩
+
+end Roo
+
+namespace Roi
+
+variable {r : Roi α}
+
+public theorem toList_eq_match [UpwardEnumerable α]
+    [LawfulUpwardEnumerable α] [Rxi.IsAlwaysFinite α] [LawfulUpwardEnumerable α] :
+    r.toList = match UpwardEnumerable.succ? r.lower with
+      | none => []
+      | some next => next :: (next<...*).toList := by
+  rw [Internal.toList_eq_toList_iter, Rxi.Iterator.toList_eq_match]; rfl
+
+public theorem toList_eq_nil_iff [UpwardEnumerable α] [LawfulUpwardEnumerable α]
+    [Rxi.IsAlwaysFinite α] [LawfulUpwardEnumerable α] :
+    r.toList = [] ↔ (UpwardEnumerable.succ? r.lower).isNone := by
+  rw [Internal.toList_eq_toList_iter, Rxi.Iterator.toList_eq_match, Internal.iter]
+  simp only
+  split <;> rename_i heq <;> simp [heq]
+
+public theorem mem_toList_iff_mem [LT α] [DecidableLT α] [UpwardEnumerable α]
+    [LawfulUpwardEnumerable α] [Rxi.IsAlwaysFinite α] [LawfulUpwardEnumerable α]
+    [LawfulUpwardEnumerableLT α] {a : α} : a ∈ r.toList ↔ a ∈ r := by
+  rw [Internal.toList_eq_toList_iter, Iter.mem_toList_iff_isPlausibleIndirectOutput,
+    Internal.isPlausibleIndirectOutput_iter_iff]
+
+-- public theorem BoundedUpwardEnumerable.init?_succ?_closed [UpwardEnumerable α]
+--     [LawfulUpwardEnumerable α] {lower lower' : Bound .closed α}
+--     (h : UpwardEnumerable.succ? lower = some lower') :
+--     init? lower' = (init? lower).bind UpwardEnumerable.succ? := by
+--   cases h : init? lower <;> rename_i ilower <;> cases h' : init? lower' <;> rename_i ilower'
+--   · simp
+--   · simp [init?] at h
+--   · simp [init?] at h'
+--   · simp_all [init?]
+
+-- @[deprecated BoundedUpwardEnumerable.init?_succ?_closed (since := "2025-08-22")]
+-- public theorem BoundedUpwardEnumerable.Closed.init?_succ [UpwardEnumerable α]
+--     [LawfulUpwardEnumerable α] {lower lower' : Bound .closed α}
+--     (h : UpwardEnumerable.succ? lower = some lower') :
+--     init? lower' = (init? lower).bind UpwardEnumerable.succ? :=
+--   init?_succ?_closed h
+
+public theorem pairwise_toList_upwardEnumerableLt
+    [UpwardEnumerable α] [LawfulUpwardEnumerable α] [Rxi.IsAlwaysFinite α] :
+    r.toList.Pairwise (fun a b => UpwardEnumerable.LT a b) := by
+  rw [Internal.toList_eq_toList_iter]
+  apply Rxi.Iterator.pairwise_toList_upwardEnumerableLt
+
+public theorem pairwise_toList_ne
+    [UpwardEnumerable α] [LawfulUpwardEnumerable α] [Rxi.IsAlwaysFinite α] :
+    r.toList.Pairwise (fun a b => a ≠ b) :=
+  List.Pairwise.imp (fun hlt => UpwardEnumerable.ne_of_lt hlt) pairwise_toList_upwardEnumerableLt
+
+public theorem pairwise_toList_lt [LT α] [UpwardEnumerable α] [LawfulUpwardEnumerable α]
+    [LawfulUpwardEnumerableLT α] [Rxi.IsAlwaysFinite α] :
+    r.toList.Pairwise (fun a b => a < b) :=
+  List.Pairwise.imp
+    (fun hlt => (LawfulUpwardEnumerableLT.lt_iff ..).mpr hlt) pairwise_toList_upwardEnumerableLt
+
+public theorem pairwise_toList_le [LE α] [UpwardEnumerable α] [LawfulUpwardEnumerable α]
+    [LawfulUpwardEnumerableLE α] [Rxi.IsAlwaysFinite α] :
+    r.toList.Pairwise (fun a b => a ≤ b) :=
+  pairwise_toList_upwardEnumerableLt
+    |> List.Pairwise.imp UpwardEnumerable.le_of_lt
+    |> List.Pairwise.imp (fun hle => (UpwardEnumerable.le_iff ..).mpr hle)
+
+-- public theorem mem_Roi_succ_succ_iff [LE α] [DecidableLE α] [UpwardEnumerable α]
+--     [LinearlyUpwardEnumerable α] [LawfulUpwardEnumerableLE α] [InfinitelyUpwardEnumerable α]
+--     [HasFiniteRanges .open α] [LawfulUpwardEnumerable α] [LawfulOpenUpperBound α]
+--     {lower : Bound .closed α} {upper : Bound .open α} {a : α} :
+--     (a ∈ (succ lower)...(succ upper)) ↔ ∃ a', a = succ a' ∧ a' ∈ lower...upper := by
+--   simp [Membership.mem, LawfulUpwardEnumerableLowerBound.isSatisfied_iff,
+--     init?, LawfulOpenUpperBound.isSatisfied_iff_le]
+--   rw [← Option.some_get (InfinitelyUpwardEnumerable.isSome_succ? _)]
+--   simp only [Option.some.injEq, ← UpwardEnumerable.succ.eq_def]
+--   simp
+--   constructor
+--   · rintro ⟨⟨n, hn⟩, h⟩
+--     rw [succMany?_eq_some_iff_succMany, ← succMany_one, ← succMany_add, Nat.add_comm, succMany_add,
+--       succMany_one] at hn
+--     rw [← hn]
+--     refine ⟨succMany n lower, rfl, ?_, ?_⟩
+--     · exact ⟨n, by simp [succMany_eq_get]⟩
+--     · obtain ⟨m, hm⟩ := h
+--       refine ⟨m, ?_⟩
+--       rw [succMany?_eq_some_iff_succMany] at hm ⊢
+--       rwa [← hn, ← succMany_one, ← succMany_add, Nat.add_comm, succMany_add, succMany_one,
+--         succ_eq_succ_iff] at hm
+--   · rintro ⟨a', rfl, hl, hu⟩
+--     simp [UpwardEnumerable.succ_le_succ_iff, UpwardEnumerable.succ_lt_succ_iff]
+--     exact ⟨hl, hu⟩
+
+public theorem mem_succ_iff [LT α] [UpwardEnumerable α]
+    [LinearlyUpwardEnumerable α] [LawfulUpwardEnumerableLT α]
+    [InfinitelyUpwardEnumerable α] [Rxi.IsAlwaysFinite α] [LawfulUpwardEnumerable α] {lo a : α} :
+    (a ∈ (succ lo)<...*) ↔ ∃ a', a = succ a' ∧ a' ∈ lo<...* := by
+  simp [Membership.mem, UpwardEnumerable.lt_iff]
+  constructor
+  · intro h
+    obtain ⟨a', rfl, ha'⟩ := UpwardEnumerable.exists_of_succ_lt h
+    exact ⟨a', rfl, UpwardEnumerable.succ_lt_succ_iff.mp h⟩
+  · rintro ⟨a', rfl, hlt⟩
+    exact UpwardEnumerable.succ_lt_succ_iff.mpr hlt
+
+public theorem succ_mem_succ_succ_iff [LT α] [UpwardEnumerable α]
+    [LinearlyUpwardEnumerable α] [LawfulUpwardEnumerableLT α]
+    [InfinitelyUpwardEnumerable α] [Rxi.IsAlwaysFinite α] [LawfulUpwardEnumerable α] {lo a : α} :
+    (succ a ∈ (succ lo)<...*) ↔ a ∈ lo<...* := by
+  simp [mem_succ_iff, UpwardEnumerable.succ_inj]
+
+-- public theorem toList_Roi_succ_succ_eq_map [UpwardEnumerable α] [SupportsLowerBound .closed α]
+--     [LinearlyUpwardEnumerable α] [InfinitelyUpwardEnumerable α] [SupportsUpperBound .open α]
+--     [HasFiniteRanges .open α] [LawfulUpwardEnumerable α] [LawfulOpenUpperBound α]
+--     [LawfulUpwardEnumerableLowerBound .closed α] [LawfulUpwardEnumerableUpperBound .open α]
+--     {lower : Bound .closed α} {upper : Bound .open α} :
+--     ((succ lower)...(succ upper)).toList =
+--       (lower...upper).toList.map succ := by
+--   apply eq_of_pairwise_lt_of_mem_iff_mem (lt := UpwardEnumerable.LT) (asymm := ?_)
+--   · apply pairwise_toList_upwardEnumerableLt
+--   · apply List.Pairwise.map (R := UpwardEnumerable.LT) (S := UpwardEnumerable.LT)
+--     · intro a b
+--       exact UpwardEnumerable.succ_lt_succ_iff.mpr
+--     · apply pairwise_toList_upwardEnumerableLt
+--   · simp only [List.mem_map, mem_toList_iff_mem]
+--     intro a
+--     rw [mem_Roi_succ_succ_iff]
+--     constructor
+--     · rintro ⟨a, rfl, h⟩
+--       exact ⟨a, h, rfl⟩
+--     · rintro ⟨a, h, h'⟩
+--       exact ⟨_, h'.symm, h⟩
+--   · exact ⟨fun _ _ => UpwardEnumerable.not_gt_of_lt⟩
+
+public theorem toList_succ_succ_eq_map [LT α] [DecidableLT α]
+    [UpwardEnumerable α] [LinearlyUpwardEnumerable α]
+    [InfinitelyUpwardEnumerable α] [Rxi.IsAlwaysFinite α]
+    [LawfulUpwardEnumerable α] [LawfulUpwardEnumerableLT α] {lo : α} :
+    ((succ lo)<...*).toList = (lo<...*).toList.map succ := by
+  apply eq_of_pairwise_lt_of_mem_iff_mem (lt := UpwardEnumerable.LT)
+  · exact pairwise_toList_upwardEnumerableLt
+  · apply List.Pairwise.map (R := UpwardEnumerable.LT) (S := UpwardEnumerable.LT)
+    · exact fun _ _ => UpwardEnumerable.succ_lt_succ_iff.mpr
+    · exact pairwise_toList_upwardEnumerableLt
+  · simp [List.mem_map, mem_toList_iff_mem, mem_succ_iff, eq_comm, and_comm]
+
+public theorem forIn'_eq_forIn'_toList [LT α] [DecidableLT α]
+    [UpwardEnumerable α] [LawfulUpwardEnumerableLT α]
+    [Rxi.IsAlwaysFinite α] [LawfulUpwardEnumerable α]
+    {γ : Type u} {init : γ} {m : Type u → Type w} [Monad m] [LawfulMonad m]
+    {f : (a : α) → a ∈ r → γ → m (ForInStep γ)} :
+    ForIn'.forIn' r init f =
+      ForIn'.forIn' r.toList init (fun a ha acc => f a (mem_toList_iff_mem.mp ha) acc) := by
+  simp [Internal.forIn'_eq_forIn'_iter, Internal.toList_eq_toList_iter,
+    Iter.forIn'_eq_forIn'_toList]
+
+public theorem forIn'_toList_eq_forIn' [LT α] [DecidableLT α]
+    [UpwardEnumerable α] [LawfulUpwardEnumerableLT α]
+    [Rxi.IsAlwaysFinite α] [LawfulUpwardEnumerable α]
+    {γ : Type u} {init : γ} {m : Type u → Type w} [Monad m] [LawfulMonad m]
+    {f : (a : α) → _ → γ → m (ForInStep γ)} :
+    ForIn'.forIn' r.toList init f =
+      ForIn'.forIn' r init (fun a ha acc => f a (mem_toList_iff_mem.mpr ha) acc) := by
+  simp [forIn'_eq_forIn'_toList]
+
+public theorem mem_of_mem_of_le [LT α] [UpwardEnumerable α]
+    [LawfulUpwardEnumerableLT α] [Rxi.IsAlwaysFinite α] [LawfulUpwardEnumerable α] {a b : α}
+    (hrb : UpwardEnumerable.LE r.lower b) (hmem : a ∈ b<...*) :
+    a ∈ r :=
+  UpwardEnumerable.lt_iff.mpr
+    (UpwardEnumerable.lt_of_le_of_lt hrb (UpwardEnumerable.lt_iff.mp hmem))
+
+-- public theorem SupportsLowerBound.isSatisfied_init? {sl} [UpwardEnumerable α]
+--     [SupportsLowerBound sl α] [BoundedUpwardEnumerable sl α] [LawfulUpwardEnumerable α]
+--     [LawfulUpwardEnumerableLowerBound sl α]
+--     {bound : Bound sl α} {a : α} (h : init? bound = some a) :
+--     SupportsLowerBound.IsSatisfied bound a := by
+--   simp only [LawfulUpwardEnumerableLowerBound.isSatisfied_iff]
+--   exact ⟨a, h, UpwardEnumerable.le_refl _⟩
+
+public theorem forIn'_eq_match_Roi [LT α] [DecidableLT α]
+    [UpwardEnumerable α] [LawfulUpwardEnumerableLT α]
+    [Rxi.IsAlwaysFinite α] [LawfulUpwardEnumerable α]
+    {m : Type u → Type w} [Monad m] [LawfulMonad m]
+    {γ : Type u} {init : γ} {f : (a : α) → _ → γ → m (ForInStep γ)} :
+    ForIn'.forIn' r init f = match hs : UpwardEnumerable.succ? r.lower with
+      | none => return init
+      | some next => do
+        have hlt : r.lower < next :=
+          UpwardEnumerable.lt_iff.mpr ⟨0, by simpa [UpwardEnumerable.succMany?_one] using hs⟩
+        have hle : UpwardEnumerable.LE r.lower next :=
+          ⟨1, by simpa [UpwardEnumerable.succMany?_one] using hs⟩
+        match ← f next hlt init with
+        | .yield c =>
+          ForIn'.forIn' (α := α) (β := γ) (next<...*) c
+            (fun a ha acc => f a (mem_of_mem_of_le hle ha) acc)
+        | .done c => return c := by
+  apply Eq.symm
+  rw [Internal.forIn'_eq_forIn'_iter, Iter.forIn'_eq_match_step]
+  simp only [Rxi.Iterator.step_eq_step, Rxi.Iterator.step, Internal.iter]
+  split <;> rename_i heq
+  · simp [heq]
+  · simp [*]; rfl
+
+public theorem isEmpty_iff_forall_not_mem [LT α] [DecidableLT α] [UpwardEnumerable α]
+    [Rxi.HasSize α] [Rxi.LawfulHasSize α] [LawfulUpwardEnumerableLT α] [Rxi.IsAlwaysFinite α]
+    [LawfulUpwardEnumerable α] :
+    r.isEmpty ↔ ∀ a, ¬ a ∈ r := by
+  simp only [isEmpty, Option.isNone_iff_eq_none, Membership.mem, UpwardEnumerable.lt_iff,
+    UpwardEnumerable.lt_iff_exists, not_exists]
+  constructor
+  · intro h a n hs
+    simp [UpwardEnumerable.succMany?_succ?_eq_succ?_bind_succMany?, h] at hs
+  · simp only [Option.eq_none_iff_forall_ne_some]
+    intro h a
+    simpa [UpwardEnumerable.succMany?_one] using h a 0
+
+end Roi
 
 private theorem Internal.iter_Roc_eq_iter_Rcc_of_isSome_succ?
     [LE α] [UpwardEnumerable α] [LawfulUpwardEnumerable α] {lo hi : α}
